backup

Protocol/SAMLProtocol.fst
@@ -1,19 +1,20 @@
-module Protocol
+module SamlProtocol
 
-open Network
+(*open Network*)
 
-type assertiontoken = string
+type assertiontoken = string (*Add refinements*)
+type signedtoken = string (*Add refinements*)
 type id = string
-
+type endpoint = string
 
 type Assertion =
-  | UnsignedAssertion: assertiontoken -> 
+  | UnsignedAssertion: assertiontoken -> Assertion
 
 type SamlMessage =
   | Login: uri -> SamlMessage
-  | AuthnRequest: prin -> samlmessage -> dsig -> SamlMessage
-  | ResponseMessage: uri -> SamlMessage
-  | LoginResponse: int -> SamlMessage
+  | AuthnRequest: issuer:prin -> id -> destination:endpoint -> dsig -> SamlMessage
+  | ResponseMessage: issuer:prin -> id -> inresto:id -> destination:endpoint -> Assertion -> SamlMessage
+  | LoginResponse: string -> SamlMessage
   | Failed: int -> SamlMessage
 
 type SamlStatus =
@@ -29,3 +30,4 @@ val SendSaml: prin -> SamlMessage -> unit
 val RecieveSaml: prin -> SamlMessage 
 
 val IssuerAssertion: issuer:prin -> subject:prin -> audience:prin -> inresto:id -> assertiontoken
+val AddSignatureToAssertion: assertiontoken -> dsig -> signedtoken
